\documentclass[10pt]{beamer}
\usepackage[cache=false]{minted}
\usepackage[utf8x]{inputenc}
\usepackage{hyperref}
\usepackage{fontawesome}
\usepackage{graphicx}
\usepackage[english,ngerman]{babel}
\usepackage{bussproofs}

% ------------------------------------------------------------------------------
% Use the beautiful metropolis beamer template
% ------------------------------------------------------------------------------
\usepackage[T1]{fontenc}
\usepackage{fontawesome}
\usepackage{FiraSans}
\newtheorem{defin}{Definition}
\newtheorem{theor}{Theorem}
\newtheorem{prop}{Proposition}
\mode<presentation>
{
  \usetheme[progressbar=foot,numbering=fraction,background=light]{metropolis}
  \usecolortheme{default} % or try albatross, beaver, crane, ...
  \usefonttheme{default}  % or try serif, structurebold, ...
  \setbeamertemplate{navigation symbols}{}
  \setbeamertemplate{caption}[numbered]
  %\setbeamertemplate{frame footer}{My custom footer}
}

% ------------------------------------------------------------------------------
% beamer doesn't have texttt defined, but I usually want it anyway
% ------------------------------------------------------------------------------
\let\textttorig\texttt
\renewcommand<>{\texttt}[1]{%
  \only#2{\textttorig{#1}}%
}

% ------------------------------------------------------------------------------
% minted
% ------------------------------------------------------------------------------


% ------------------------------------------------------------------------------
% tcolorbox / tcblisting
% ------------------------------------------------------------------------------
\usepackage{xcolor}
\definecolor{codecolor}{HTML}{FFC300}

\usepackage{tcolorbox}
\tcbuselibrary{most,listingsutf8,minted}

\tcbset{tcbox width=auto,left=1mm,top=1mm,bottom=1mm,
right=1mm,boxsep=1mm,middle=1pt}

\newtcblisting{myr}[1]{colback=codecolor!5,colframe=codecolor!80!black,listing only,
minted options={numbers=left, style=tcblatex,fontsize=\tiny,breaklines,autogobble,linenos,numbersep=3mm},
left=5mm,enhanced,
title=#1, fonttitle=\bfseries,
listing engine=minted,minted language=r}


% ------------------------------------------------------------------------------
% Listings
% ------------------------------------------------------------------------------
\definecolor{mygreen}{HTML}{37980D}
\definecolor{myblue}{HTML}{0D089F}
\definecolor{myred}{HTML}{98290D}

\usepackage{listings}

% the following is optional to configure custom highlighting
\lstdefinelanguage{XML}
{
  morestring=[b]",
  morecomment=[s]{<!--}{-->},
  morestring=[s]{>}{<},
  morekeywords={ref,xmlns,version,type,canonicalRef,metr,real,target}% list your attributes here
}

\lstdefinestyle{myxml}{
language=XML,
showspaces=false,
showtabs=false,
basicstyle=\ttfamily,
columns=fullflexible,
breaklines=true,
showstringspaces=false,
breakatwhitespace=true,
escapeinside={(*@}{@*)},
basicstyle=\color{mygreen}\ttfamily,%\footnotesize,
stringstyle=\color{myred},
commentstyle=\color{myblue}\upshape,
keywordstyle=\color{myblue}\bfseries,
}


% ------------------------------------------------------------------------------
% The Document
% ------------------------------------------------------------------------------
\title{Functional programming, Seminar No. 5}
\author{Danya Rogozin \\ Institute for Information Transmission Problems, RAS \\ Serokell O\"{U}}
\date{Higher School of Economics \\ The Faculty of Computer Science}

\begin{document}

\maketitle

\begin{frame}
\frametitle{Today}
We will study
\begin{center}
\includegraphics[scale=0.12]{retriever.jpeg}
\end{center}
\end{frame}


\section{Foldable}

\begin{frame}[fragile]
\frametitle{\verb"Semigroup" and \verb"Monoid": the definition}

In this subsection, we study the generalisation of folds with the type class called \verb"Foldable".
For that, we have a look at the classes called \verb"Semigroup" and \verb"Monoid". Here are the definition.

\begin{minted}{haskell}
class Semigroup a where
  (<>) :: a -> a -> a

class Semigroup a => Monoid a where
  mempty :: a
  mappend :: a -> a -> a
  mappend = (<>)
  mconcat :: [a] -> a
  mconcat = foldr mappend mempty
\end{minted}
\end{frame}

\begin{frame}[fragile]
  \frametitle{\verb"Semigroup" and \verb"Monoid": the laws}

  The operation in a semigroup should associative and \verb"mempty" is the neutral element:
  \begin{minted}{haskell}
  a <> (b <> c) == (a <> b) <> c
  a <> mempty == a = mempty <> a
  \end{minted}
  \begin{itemize}
  \item NOTE BENE: every \verb"Semigroup"/\verb"Monoid" instance should obey these laws.
  \item The compiler is not capable of proving such properties (note that tests $\neq$ proofs), so programmers have to ensure that required laws are valid for such instances.
  \item The moral is that declaring a \verb"Semigroup" instance where the operations happens to be non-associative is \emph{mauvais go\^{u}t}.
\end{itemize}
\end{frame}

\begin{frame}[fragile]
\frametitle{The \verb"Monoid" instances}
\begin{minted}{haskell}
instance Semigroup [a] where
  (<>) = (++)

instance Monoid [a] where
  mempty = []
\end{minted}

\verb"(++)" is associative operation and \verb"[]" is neutral. A semiformal proof:
\begin{minted}{haskell}
[] ++ (ys ++ zs) = ys ++ zs = ([] ++ ys) ++ zs

(x : xs) ++ (ys ++ zs) =
  x : (xs ++ (ys ++ zs)) = -- IH
  x : ((xs ++ ys) ++ zs) =
  (x : (xs ++ ys)) ++ zs =
  (x : (xs ++ ys)) ++ zs
\end{minted}
\end{frame}

\begin{frame}[fragile]
\frametitle{Numbers and Booleans as monoids}

\begin{minted}{haskell}
newtype Sum a = Sum { getSum :: a }
  deriving (Show, Eq, Ord)

instance Num a => Semigroup (Sum a) where
  Sum a <> Sum b = Sum (a + b)

instance Num a => Monoid (Sum a) where
  mempty = Sum 0
\end{minted}

\vspace{\baselineskip}

One has the \verb"Monoid" instance for any numerical type with the product as a binary operation.
For that one needs to introduce the following new type because the same type cannot have two different instances.

\begin{minted}{haskell}
newtype Sum a = Sum { getSum :: a }
  deriving (Show, Eq, Ord)
\end{minted}
\end{frame}

\begin{frame}[fragile]
\frametitle{Numbers and Booleans as monoids}

\begin{minted}{haskell}
newtype All = All { getAll :: Bool }
  deriving (Show, Eq, Show)

instance Semigroup All where
  All a <> All b = All (a && b)

instance Monoid All where
  mempty = All True
\end{minted}

\vspace{\baselineskip}

The similar for disjunction by putting \verb"a <> b = a || b" and \verb"mempty = False".
\end{frame}

\begin{frame}[fragile]
\frametitle{Foldable: Motivation}

\begin{itemize}
\item Before we took a look at such fold functions as \verb"foldr"
\begin{minted}{haskell}
  foldr :: (a -> b -> b) -> b -> [a] -> b
  foldr _ ini [] = []
  foldr f ini (x : xs) = f x (foldr f ini xs)
\end{minted}
\item One may generalise the idea of folding to consider a broader class of foldable data structures
\end{itemize}

\end{frame}

\begin{frame}[fragile]
\frametitle{The \verb"Foldable" type class}
\begin{minted}{haskell}
class Foldable t where
  {-# MINIMAL foldMap | foldr #-}
  foldMap :: Monoid m => (a -> m) -> t a -> m
  foldMap f = foldr (mappend . f) mempty

  foldr :: (a -> b -> b) -> b -> t a -> b
  foldr f z t = appEndo (foldMap (Endo . f) t) z
\end{minted}
where
\begin{minted}{haskell}
  newtype Endo a = Endo { appEndo :: a -> a }
\end{minted}
\end{frame}

\begin{frame}[fragile]
\frametitle{Useful functions for foldable data types}
Here we provide type signatures only:
\begin{minted}{haskell}
toList :: Foldable t => t a -> [a]

null :: Foldable => t a -> Bool

length :: Foldable t => t a -> Int

elem :: (Eq a, Foldable t) => a -> t a -> Bool

maximum :: (Ord a, Foldable t) => t a -> a

sum, product :: (Num a, Foldable t) => t a -> a
\end{minted}
\end{frame}

\begin{frame}[fragile]
\frametitle{Foldable instances.}

\begin{minted}{haskell}
instance Foldable [] where
    elem    = List.elem
    foldl   = List.foldl
    foldr   = List.foldr
    length  = List.length
    maximum = List.maximum
    product = List.product
\end{minted}
\end{frame}

\begin{frame}[fragile]
\frametitle{Foldable instances. Other examples}

\begin{minted}{haskell}
instance Foldable (Either a) where
    foldMap _ (Left _) = mempty
    foldMap f (Right y) = f y

    foldr _ z (Left _) = z
    foldr f z (Right y) = f y z

    length (Left _)  = 0
    length (Right _) = 1

    null             = isLeft

instance Foldable ((,) a) where
    foldMap f (_, y) = f y
    foldr f z (_, y) = f y z
\end{minted}
\end{frame}

\begin{frame}[fragile]
\frametitle{Foldable instances. Other examples}

\begin{minted}{haskell}
instance Foldable NonEmpty
instance Foldable Set
instance Foldable (Map k)
instance Foldable (Array i)
instance Foldable Vector
\end{minted}
\end{frame}

\section{Functor}

\begin{frame}[fragile]
\frametitle{Motivation}

\begin{itemize}
\item Let us have a look at the following functions:
    \begin{minted}{haskell}
    map :: (a -> b) -> [a] -> [b]
    map _ [] = []
    map f (x : xs) = f x : map f xs

    mapMaybe :: (a -> b) -> Maybe a -> Maybe b
    mapMaybe _ Nothing = Nothing
    mapMaybe f (Just x) = Just (f x)
    \end{minted}
\item These function are similar. Here we have an unary function that we carry through a element of a parametrised type.
\item We generalise that with the type class \verb"Functor".
\end{itemize}
\end{frame}

\begin{frame}[fragile]
\frametitle{Functor: the definition and instances}
\begin{minted}{haskell}
class Functor (f :: * -> *) where
  fmap :: (a -> b) -> (f a -> f b)

instance Functor Maybe where
  fmap _ Nothing = Nothing
  fmap f (Just x) = Just (f x)

instance Functor [] where
  fmap _ [] = []
  fmap f (x : xs) = f x : map f xs
\end{minted}
\end{frame}

\begin{frame}[fragile]
\frametitle{The full definition of \verb"Functor"}

\begin{minted}{haskell}
class Functor (f :: * -> *) where
  fmap        :: (a -> b) -> f a -> f b
  (<$)        :: a -> f b -> f a
  (<$)        =  fmap . const

infixl 4 <$>, <$

(<$>) :: Functor f => (a -> b) -> f a -> f b
(<$>) = fmap

void :: Functor f => f a -> f ()
void x = () <$ x
\end{minted}
\end{frame}

\begin{frame}[fragile]
\frametitle{Another example of a \verb"Functor" instance}

\begin{minted}{haskell}
import Data.Functor

data Tree a = Leaf a | Node (Tree a) a (Tree a)
  deriving Show

instance Functor Tree where
  fmap f (Leaf a) = Leaf (f a)
  fmap f (Node ls a rs) = Node (fmap f ls) (f a) (fmap f rs)

left = Node (Leaf 2) 3 (Leaf 5)
right = Node (Leaf 5) 7 (Leaf 11)
tree = Node left 13 right

treeWord = (\x -> show x ++ show x) <$> tree
voidTree = void tree
constTree = "Anna" <$ treeWord
\end{minted}

\end{frame}

\begin{frame}[fragile]
\frametitle{The example of a \verb"Functor" instance. The \verb"DeriveFunctor" extension}

One may derive the \verb"Functor" instance automatically for some data types.

\begin{minted}{haskell}
{-# LANGUAGE DeriveFunctor #-}

import Data.Functor

data Tree a = Leaf a | Node (Tree a) a (Tree a)
  deriving (Show, Functor)
\end{minted}

\vspace{\baselineskip}

The derived instance in this example is equivalent to our version above.
\end{frame}

\begin{frame}[fragile]
\frametitle{\verb"Functor" instances for two-parametric data types}

Let us take a look at the \verb"Functor" for type constructors that have
kind \verb"* -> * -> *". The first argument of such a constructor is fixed.

\begin{minted}{haskell}
instance Functor ((,) a) where
  fmap f (x,y) = (x, f y)

instance Functor ((->) r) where
  fmap = (.)

instance Functor (Either a) where
  fmap _ (Left x) = Left x
  fmap f (Right y) = Right (f y)
\end{minted}
\end{frame}

\begin{frame}[fragile]
\frametitle{The \verb"Functor" laws}

Any \verb"Functor" instance is expected to satisfy the following axioms:

\begin{minted}{haskell}

fmap id fx = fx

fmap (f . g) fx = (fmap f . fmap g) fx
\end{minted}
\end{frame}

\begin{frame}[fragile]
\frametitle{The \verb"Functor" laws. Example}
Let us check that the list data type is really a functor.

\begin{minted}{haskell}

fmap id [] = map id [] = []
fmap id (x : xs) =
  id x : fmap id xs =
  x : fmap id xs =      -- IH
  x : xs

fmap (f . g) [] = []
fmap (f . g) (x : xs) =
  (f . g) x : fmap (f . g) xs =   -- IH
  (f . g) x : (fmap f . fmap g) xs =
  f (g x) : fmap f (fmap g xs)
\end{minted}
\end{frame}

\section{Applicative functors}

\begin{frame}[fragile]
\frametitle{Motivation}

It is clear that we would like to have something like \verb"fmap" for functions of an arbitrary arity:
\begin{minted}{haskell}
fmap2
  :: (a -> b -> c)
  -> f a -> f b -> f c
fmap3
  :: (a -> b -> c -> d)
  -> f a -> f b -> f c -> f d
fmap4
  :: (a -> b -> c -> d -> e)
  -> f a -> f b -> f c -> f d -> e
...
\end{minted}
We cannot do that using only \verb"fmap" for unary functions.
\end{frame}

\begin{frame}[fragile]
\frametitle{The \verb"Applicative" class}

\begin{minted}{haskell}
class Functor f => Applicative f where
    {-# MINIMAL pure, ((<*>) | liftA2) #-}
    pure :: a -> f a

    (<*>) :: f (a -> b) -> f a -> f b
    (<*>) = liftA2 ($)

    liftA2 :: (a -> b -> c) -> f a -> f b -> f c
    liftA2 f x = (<*>) (fmap f x)
\end{minted}
\end{frame}

\begin{frame}[fragile]
\frametitle{The \verb"Applicative" class. A couple of examples}
\begin{minted}{haskell}
instance Applicative Maybe where
  pure = Just
  Nothing <*> _ = Nothing
  _ <*> Nothing = Nothing
  Just f <*> Just x = Just (f x)

instance Applicative [] where
  pure x = [x]
  fs <*> fx = [ f x | f <- fs, x <- xs]
\end{minted}
\end{frame}

\begin{frame}[fragile]
\frametitle{The \verb"Applicative" laws}
\begin{minted}{haskell}
fmap f x = pure f <*> x

pure id <*> v = v  -- identity

pure (.) <*> u <*> v <*> w = u <*> (v <*> w) -- composition

pure f <*> pure x = pure (f x) -- homomorphism

u <*> pure y = pure (\f -> f y) <*> u -- interchange
\end{minted}
\end{frame}

\begin{frame}[fragile]
\frametitle{The \verb"Applicative" class. Another \verb"Applicative" instance for lists}
\begin{itemize}
\item The list data type might have an alternative \verb"Applicative" instance
\item Recall the function \verb"zipWith":
\begin{minted}{haskell}
zipWith :: (a -> b -> c) -> [a] -> [b] -> [c]
zipWith _ [] _ = []
zipWith _ _ [] = []
zipWith f (x:xs) (y:ys) = f x y : zipWith f xs ys
\end{minted}
\item The signature of \verb"zipWith" corresponds to the signature of \verb"liftA2"
\item On the other hand, as we've already said, we cannot have two instances for the same data type
\end{itemize}
\end{frame}

\begin{frame}[fragile]
\frametitle{The \verb"Applicative" class. Another \verb"Applicative" instance for lists}
\begin{minted}{haskell}
newtype ZipList a = ZipList { getZipList :: [a] }

instance Functor ZipList where
  fmap f = ZipList . getZipList . fmap f

instance Applicative ZipList where
  liftA2 f (ZipList xs) (ZipList ys) =
    ZipList (zipWith f xs ys)
  zipF <*> zipX = liftA2 ($)
  pure = ???
\end{minted}

How to implement \verb"pure" and preverse the applicative laws?
If we define \verb"pure" as below, that would break all those axioms.
\begin{minted}{haskell}
  pure x = ZipList [x]
\end{minted}

\end{frame}

\begin{frame}[fragile]
\frametitle{The \verb"Applicative" class. Another \verb"Applicative" instance for lists}

\begin{itemize}
\item Here is the proper instance:
\begin{minted}{haskell}
instance Applicative ZipList where
  liftA2 f (ZipList xs) (ZipList ys) =
    ZipList (zipWith f xs ys)
  zipF <*> zipX = liftA2 ($)
  pure a = ZipList $ iterate x
    where iterate x = x : iterate x
\end{minted}
\end{itemize}
\end{frame}

\begin{frame}[fragile]
\frametitle{\verb"Applicative" instance for tuples}

The \verb"Monoid" type class allows one to have the \verb"Applicative" instance for
tuples as follows:

\begin{minted}{haskell}
instance Monoid a => Applicative ((,) a) where
  pure x = (mempty x, x)
  (a, f) <*> (b, x) = (a <> b, f x)
\end{minted}

\end{frame}

\section{Traversable}

\begin{frame}[fragile]
\frametitle{The motivating example}
\begin{minted}{haskell}
dist :: Applicative f => [f a] -> f [a]
dist [] = pure []
dist (x : xs) = liftA2 (:) x (dist xs)
\end{minted}

\begin{minted}{haskell}
> dist (Just <$> [1,2,4])
Just [1,2,4]
> dist [Just 1, Nothing]
Nothing
> getZipList $ dist $ map ZipList [[1,2,3], [4,5,6], [7,8,9]]
[[1,4,7],[2,5,8],[3,6,9]]
\end{minted}

\end{frame}

\begin{frame}[fragile]
\frametitle{The \verb"Traversable" definition}

According to the documentation, \verb"Traversable" describes ``functors representing data structures that can be traversed from left to right''.

\begin{minted}{haskell}
class (Functor t, Foldable t) => Traversable t where
  traverse :: Applicative f => (a -> f b) -> t a -> f (t b)
  traverse f = sequenceA . fmap f

  sequenceA :: Applicative f => t (f a) -> f (t a)
  sequenceA = traverse id
  {-# MINIMAL traverse | sequenceA #-}
\end{minted}
\end{frame}

\begin{frame}[fragile]
\frametitle{The \verb"Traversable" instances}

\begin{minted}{haskell}
instance Travesable Maybe where
  traverse _ Nothing = Nothing
  traverse f (Just x) = Just <$> f x

instace Traversable [] where
  traverse _ g = foldr consF (pure [])
    where
      consF x ys = liftA2 (:) (g x) ys
\end{minted}
\end{frame}

\section{Summary}

\begin{frame}
\frametitle{Summary}

Today we
\begin{itemize}
\item introduced such type classes as \verb"Functor", \verb"Applicative", \verb"Monoid", \verb"Foldable",
and \verb"Traversable"
\end{itemize}

\onslide<2->{
  Next time, we will
  \begin{itemize}
  \item study monads!
  \end{itemize}
}
\end{frame}

\end{document}
